Cpc/TypePreservation/Support.lean
@@ -680,6 +680,12 @@ inductive supported_preservation_term : SmtTerm -> Prop
       supported_preservation_term (SmtTerm.Apply SmtTerm.sbv_to_int t)
   | dt_cons (s : smt_lit_String) (d : SmtDatatype) (i : smt_lit_Nat) :
       supported_preservation_term (SmtTerm.DtCons s d i)
+  | dt_sel {s : smt_lit_String} {d : SmtDatatype} {i j : smt_lit_Nat} {x : SmtTerm}
+      (ht : term_has_non_none_type (SmtTerm.Apply (SmtTerm.DtSel s d i j) x))
+      (hT : type_inhabited (__smtx_typeof (SmtTerm.Apply (SmtTerm.DtSel s d i j) x)))
+      (htx : term_has_non_none_type x)
+      (hsx : supported_preservation_term x) :
+      supported_preservation_term (SmtTerm.Apply (SmtTerm.DtSel s d i j) x)
   | dt_tester (s : smt_lit_String) (d : SmtDatatype) (i : smt_lit_Nat) (x : SmtTerm) :
       supported_preservation_term (SmtTerm.Apply (SmtTerm.DtTester s d i) x)
   | apply {f x : SmtTerm}
